%!TEX program = xelatex
\documentclass[11pt, a4paper]{article}

\usepackage{amsmath}
\usepackage{amssymb}
\usepackage{graphicx}

\title{ps4-4-sol}
\author{virusdoll}

\begin{document}
    \maketitle

    % problem (a)
    \section*{(a)}
    
    \begin{align*}
        \ell(W)
        & = \sum^m_{i=1} \big( \log |W| + \sum^d_{j=1} \log g' (w^T_j x^{(i)}) \big) \\
        & = \sum^m_{i=1} \big(
            \log |W|
            + \sum^d_{j=1} \log (2 \pi)^{\frac{1}{2}} \exp (- \frac{1}{2} (w^T_j x^{(i)})^2)
        \big) \\
        & = \sum^m_{i=1} \big(
            \log |W|
            + \sum^d_{j=1} - \frac{1}{2} \log 2 \pi - \frac{1}{2} (w^T_j x^{(i)})^2
        \big) \\
        & = \sum^m_{i=1} \big(
            \log |W|
            - \frac{1}{2} d \log 2 \pi
            - \frac{1}{2} {x^{(i)}}^T W^T W x^{(i)}
        \big)
    \end{align*}

    \begin{align*}
        \nabla_W \ell(W)
        & = \nabla_W \sum^m_{i=1} \big(
            \log |W|
            - \frac{1}{2} d \log 2 \pi
            - \frac{1}{2} {x^{(i)}}^T W^T W x^{(i)}
        \big) \\
        & = \sum^m_{i=1} \big(
            W^{-T}
            - \frac{1}{2} \nabla_W \ \text{tr} \ {x^{(i)}}^T W^T W x^{(i)}
        \big) \\
        & = \sum^m_{i=1} \big(
            W^{-T}
            - \frac{1}{2} \nabla_W \ \text{tr} \ W^T W x^{(i)} {x^{(i)}}^T
        \big) \\
        & = \sum^m_{i=1} \big( W^{-T} - W x^{(i)} {x^{(i)}}^T \big) \\
        & = n W^{-T} - W X^T X
    \end{align*}

    Let $\nabla_W \ell(W) = 0$, then
    \begin{align*}
        n W^{-T} & = W X^T X \\
        W^T W & = n (X^T X)^{-1}
    \end{align*}

    Let $R$ be an arbitrary orthogonal matrix, then
    \begin{align*}
        (RW)^T RW & = W^T R^T R W \\
        & = W^T I W \\
        & = W^T W \qquad \text{for any} \ R
    \end{align*}

    So the result of $W$ can be any of the $RW$.

    % problem (b)
    \section*{(b)}
    
    For $x^{(i)}$, we have
    \begin{align*}
        \nabla_W \ell(W)
        & = \nabla_W \big( \log |W| + \sum^d_{j=1} \log g' (w^T_j x^{(i)}) \big) \\
        & = \nabla_W \big(
            \log |W| + \sum^d_{j=1} \log \frac{1}{2} \exp (-|w^T_j x^{(i)}|)
        \big) \\
        & = \nabla_W \big(
            \log |W| + \sum^d_{j=1} \log \frac{1}{2} -|w^T_j x^{(i)}|
        \big) \\
        & = \nabla_W \big(
            \log |W| + d \log \frac{1}{2} - \sum^d_{j=1} |w^T_j x^{(i)}|
        \big) \\
        & = W^{-T} - \nabla_W \sum^d_{j=1} |w^T_j x^{(i)}| \\
        & = W^{-T} - \left[ \begin{array}{c}
            \frac{\partial}{\partial w^T_1} |w^T_1 x^{(i)}| \\
            \cdots \\
            \frac{\partial}{\partial w^T_d} |w^T_d x^{(i)}| \\
        \end{array}
        \right] \\
        & = W^{-T} - \left[ \begin{array}{c}
            \text{sign}(w^T_1 x^{(i)}) {x^{(i)}}^T \\
            \cdots \\
            \text{sign}(w^T_d x^{(i)}) {x^{(i)}}^T \\
        \end{array}
        \right] \\
        & = W^{-T} - \text{sign}(W^T x^{(i)}) {x^{(i)}}^T
    \end{align*}

    Then,
    $$W := W + \alpha \big( W^{-T} - \text{sign}(W^T x^{(i)}) {x^{(i)}}^T \big)$$

\end{document}